KmsArnIdentifier.dfy
@@ -45,12 +45,11 @@ type AccountString = s:string | AccountString?(s) witness *
 // The resource id MUST be a non-empty string 
 // this seq<string> length is 2, x[0] is key, x[1] is ID.
 
-predicate ResourceSeqStr?(x:seq<string>)
+predicate KmsResource?(x:string, y:string)
 {
-    |x| == 2 && (x[0]=="alias" || x[0] == "key") && |x[1]| != 0
+    (x=="alias" ||x == "key") && |y| != 0
 }
 
-type ResourceSeqStr = x:seq<string> | ResourceSeqStr?(x) witness *
 
 datatype ARN = ARN(
     arnLiteral: string,
@@ -58,12 +57,29 @@ datatype ARN = ARN(
     service: string,
     region: string,
     account: string,
-    resource: seq<string>
+    resource: Resource
 )
 
 
 
-type KmsArn = a: ARN | KmsArn?(a) witness *
+// type KmsArn = a: ARN | KmsArn?(a) witness *
+
+
+type resourceType = s:string | s == "alias" || s == "key" witness *
+
+type ResourceId = s:string | |s| != 0 witness *
+
+
+
+datatype Resource = Resource(
+    rtype : string,
+    id : string
+)
+
+datatype KmsResource = KmsResource(
+    rtype : resourceType,
+    id : ResourceId
+)
 
 datatype KmsArnDatatype = KmsArnDatatype(
     arnLiteral: ArnString,
@@ -71,49 +87,50 @@ datatype KmsArnDatatype = KmsArnDatatype(
     service: ServiceString,
     region: RegionString,
     account: AccountString,
-    resource: ResourceSeqStr
+    resource: KmsResource
 )
 
 
 
 
-predicate KmsArn?(a:ARN)
+// predicate KmsArn?(a:ARN)
 
-{
-    if
-        // MUST start with string arn
-        && a.arnLiteral == "arn"
+// {
+//     if
+//         // MUST start with string arn
+//         && a.arnLiteral == "arn"
 
-        // The partition MUST be a non-empty
-        && |a.partition| !=0
+//         // The partition MUST be a non-empty
+//         && |a.partition| !=0
 
-        // The service MUST be the string kms
-        && a.service == "kms"
+//         // The service MUST be the string kms
+//         && a.service == "kms"
 
-        //The account MUST be a non-empty string
-        && |a.account| != 0
+//         //The account MUST be a non-empty string
+//         && |a.account| != 0
 
-        // The region MUST be a non-empty string
-        && |a.region| !=0
+//         // The region MUST be a non-empty string
+//         && |a.region| !=0
 
-        // then it leads to resource type to be key or alias, and both id cannot be empty
-        &&  |a.resource|>=2
-        &&  (
-            (&& a.resource[0] == "key"
-            && |a.resource[1]|!=0 ) 
-            || 
-            (&& a.resource[0] == "alias" 
-            && |a.resource[1]| != 0 )
-            )
-    then true
-    else false
-}
+//         // then it leads to resource type to be key or alias, and both id cannot be empty
+//         &&  |a.resource|>=2
+//         &&  (
+//             (&& a.resource[0] == "key"
+//             && |a.resource[1]|!=0 ) 
+//             || 
+//             (&& a.resource[0] == "alias" 
+//             && |a.resource[1]| != 0 )
+//             )
+//     then true
+//     else false
+// }
 
-method test()
-{
-    assert ARN("arn","aws","kms","us-east-1","2222222222222",["key","testid"]).ARN? == true;
+// method test()
+// {
+//     assert ARN("arn","aws","kms","us-east-1","2222222222222",["key","testid"]).ARN? == true;
 
-    assert KmsArn?(ARN("arn","aws","kms","us-east-1","2222222222222",["alias","testid"])) == true;
+//     assert KmsArn?(ARN("arn","aws","kms","us-east-1","2222222222222",["alias","testid"])) == true;
 
-    assert KmsArnDatatype("arn","aws","kms","us-east-1","2222222222222",["key","testid"]).KmsArnDatatype? == true;
-}
+//     assert KmsArnDatatype("arn","aws","kms","us-east-1","2222222222222",["key","testid"]).KmsArnDatatype? == true;
+
+// }
